Z_Machine.thy
@@ -19,8 +19,11 @@ lemma wp_zop [wp, code_unfold]: "wp (mk_zop P \<sigma> Q v) b = [\<lambda> \<s>.
 lemma wlp_zop [wp, code_unfold]: "wlp (mk_zop P \<sigma> Q v) b = [\<lambda> \<s>. P v \<s> \<longrightarrow> Q v \<s> \<longrightarrow> (\<sigma> v \<dagger> [\<lambda> \<s>. b \<s>]\<^sub>e) \<s>]\<^sub>e"
   by (simp add: mk_zop_def wp)
 
-lemma itree_pre [dpre]: "itree_pre (mk_zop P \<sigma> Q v) = [\<lambda> \<s>. P v \<s>]\<^sub>e"
+lemma itree_pre_zop [dpre]: "itree_pre (mk_zop P \<sigma> Q v) = [\<lambda> \<s>. P v \<s>]\<^sub>e"
   by (simp add: mk_zop_def dpre wp)
+
+lemma itree_rel_zop [rel]: "itree_rel (mk_zop P \<sigma> Q v) = {(x, z). P v x \<and> Q v x \<and> z = \<sigma> v x}"
+  by (simp add: mk_zop_def rel relcomp_unfold)
 
 text \<open> An operation can have its parameters supplied by an event, using the construct below. \<close>
 
